\documentclass[./main.tex]{subfiles}

\usepackage{amsmath}
\usepackage{mathtools}
\usepackage{commath}

\begin{document}

\chapter{Multilateration}

\begin{equation}
    \begin{dcases*}
        P_0 = 
        \begin{bmatrix}
            p_0^x & p_0^y & p_0^z
        \end{bmatrix} \\
        P_1 = 
        \begin{bmatrix}
            p_1^x & p_1^y & p_1^z
        \end{bmatrix} \\
        P_2 = 
        \begin{bmatrix}
            p_2^x & p_2^y & p_2^z
        \end{bmatrix} \\
        P_3 = 
        \begin{bmatrix}
            p_3^x & p_3^y & p_3^z
        \end{bmatrix}
    \end{dcases*}
    \label{eqn:anchor_location}
\end{equation}

\begin{equation}
    \begin{dcases*}
        r_0 \\ r_1 \\ r_2 \\ r_3
    \end{dcases*}
    \label{eqn:anchor_location}
\end{equation}

\begin{equation}
    e_x^{1\times3} = \frac{P_1 - P_0}{\norm[1]{P_1 - P_0}}
\end{equation}

\begin{equation}
    i^{1\times1} = e_x^{1\times3}.(P_2 - P_0)^{1\times3}
\end{equation}

\begin{equation}
    e_y^{1\times3} = \frac{P_2-P_0-(i*e_x)}{\norm[1]{P_2-P_0-(i*e_x)}}
\end{equation}

\begin{equation}
    e_z^{1\times3} = e_x \times e_y
\end{equation}

\begin{equation}
    d = \norm[1]{P_1 - P_0}
\end{equation}

\begin{equation}
    j^{1\times1} = e_y^{1\times3}.(P_2 - P_0)^{1\times3}
\end{equation}

\begin{equation}
    x = \frac{r_0^2 - r_1^2 + d^2}{2d}
\end{equation}

\begin{equation}
    y = r_0^2 - r_2^2 + i^2 + j^2/(2j) - \frac{i}{j}*x
\end{equation}

\end{document}